some progress

Veil/Theory/Defs.lean
@@ -42,10 +42,10 @@ abbrev RProp (α ρ σ : Type) := α -> SProp ρ σ
 
 /-! Our language is parametric over the mutable state, immutable state, and return type. -/
 set_option linter.unusedVariables false in
-abbrev VeilExecM (m : Mode) (σ ρ α : Type) := ReaderT ρ (StateT σ (ExceptT ExId DivM)) α
-abbrev VeilM (m : Mode) (σ ρ α : Type) := NonDetT (VeilExecM m σ ρ) α
+abbrev VeilExecM (m : Mode) (ρ σ α : Type) := ReaderT ρ (StateT σ (ExceptT ExId DivM)) α
+abbrev VeilM (m : Mode) (ρ σ α : Type) := NonDetT (VeilExecM m ρ σ) α
 
-abbrev VeilSpecM (σ ρ α : Type) := Cont (SProp ρ σ) α
+abbrev VeilSpecM (ρ σ α : Type) := Cont (SProp ρ σ) α
 
 abbrev BigStep (ρ σ α : Type) := ρ -> σ -> α -> σ -> Prop
 abbrev TwoState (ρ σ : Type) := ρ -> σ -> σ -> Prop
@@ -61,35 +61,35 @@ macro "[DemonFail|" t:term "]" : term =>  `(open PartialCorrectness DemonicChoic
 macro "[AngelFail|" t:term "]" : term =>  `(open TotalCorrectness AngelicChoice ExceptionAsFailure in $t)
 macro "[CanRaise" ex:term "|" t:term "]" : term =>  `(open PartialCorrectness DemonicChoice in let _ : IsHandler (ε := ExId) $ex := ⟨⟩; $t)
 
-variable {m : Mode} {σ ρ α : Type}
+variable {m : Mode} {ρ σ α : Type}
 
 section WeakestPreconditionsSemantics
 
-def VeilM.succesfullyTerminates (act : VeilM m σ ρ α) (pre : SProp ρ σ) : Prop :=
+def VeilM.succesfullyTerminates (act : VeilM m ρ σ α) (pre : SProp ρ σ) : Prop :=
   [DemonFail| triple pre act ⊤]
 
-def VeilM.preservesInvariantsOnSuccesful (act : VeilM m σ ρ α) (inv : SProp ρ σ) : Prop :=
+def VeilM.preservesInvariantsOnSuccesful (act : VeilM m ρ σ α) (inv : SProp ρ σ) : Prop :=
   [DemonSucc| triple inv act (fun _ => inv)]
 
-def VeilM.succeedsAndPreservesInvariants (act : VeilM m σ ρ α) (inv : SProp ρ σ) : Prop :=
+def VeilM.succeedsAndPreservesInvariants (act : VeilM m ρ σ α) (inv : SProp ρ σ) : Prop :=
   [DemonFail| triple inv act (fun _ => inv)]
 
-abbrev VeilM.choices (act : VeilM m σ ρ α) := ExtractNonDet WeakFindable act
+abbrev VeilM.choices (act : VeilM m ρ σ α) := ExtractNonDet WeakFindable act
 
-def VeilM.assumptions (act : VeilM m σ ρ α) (chs : act.choices) : SProp ρ σ := [DemonFail| chs.prop]
+def VeilM.assumptions (act : VeilM m ρ σ α) (chs : act.choices) : SProp ρ σ := [DemonFail| chs.prop]
 
 noncomputable
-def VeilM.run (act : VeilM m σ ρ α) (chs : act.choices) : VeilExecM m σ ρ α :=
+def VeilM.run (act : VeilM m ρ σ α) (chs : act.choices) : VeilExecM m ρ σ α :=
   act.runWeak chs
 
 end WeakestPreconditionsSemantics
 
 section TwoStateSemantics
 
-def VeilSpecM.toTwoState (spec : VeilSpecM σ ρ α) : TwoState ρ σ :=
+def VeilSpecM.toTwoState (spec : VeilSpecM ρ σ α) : TwoState ρ σ :=
   fun r₀ s₀ s₁ => spec (fun _ r s => r = r₀ ∧ s = s₁) r₀ s₀
 
-def VeilM.toTwoState (act : VeilM m σ ρ α) : TwoState ρ σ :=
+def VeilM.toTwoState (act : VeilM m ρ σ α) : TwoState ρ σ :=
   fun r₀ s₀ s₁ =>
     [AngelFail| triple (fun r s => r = r₀ ∧ s = s₀) act (fun _ r s => r = r₀ ∧ s = s₁)]
 
@@ -106,19 +106,19 @@ end TwoStateSemantics
 
 section OperationalSemantics
 
-def VeilExecM.operational (act : VeilExecM m σ ρ α) (r₀ : ρ) (s₀ : σ) (s₁ : σ) (res : Except ExId α) : Prop :=
+def VeilExecM.operational (act : VeilExecM m ρ σ α) (r₀ : ρ) (s₀ : σ) (s₁ : σ) (res : Except ExId α) : Prop :=
   match act r₀ s₀ with
   | .div => False
   | .res (.error i)   => res = .error i ∧ /- can be anything -/ s₁ = s₀
   | .res (.ok (a, s)) => res = .ok a ∧ s = s₁
 
-def VeilExecM.axiomatic (act : VeilExecM m σ ρ α) (r₀ : ρ) (s₀ : σ) (post : RProp α ρ σ) : Prop :=
+def VeilExecM.axiomatic (act : VeilExecM m ρ σ α) (r₀ : ρ) (s₀ : σ) (post : RProp α ρ σ) : Prop :=
   match act r₀ s₀ with
   | .div => False
   | .res (.error _) => False
   | .res (.ok (a, s)) => post a r₀ s
 
-def VeilExecM.operationalTriple (act : VeilExecM m σ ρ α) (pre : SProp ρ σ) (post : RProp α ρ σ) : Prop :=
+def VeilExecM.operationalTriple (act : VeilExecM m ρ σ α) (pre : SProp ρ σ) (post : RProp α ρ σ) : Prop :=
   ∀ r₀ s₀ s₁ res,
     pre r₀ s₀ ->
     act.operational r₀ s₀ s₁ res ->
@@ -131,13 +131,13 @@ end OperationalSemantics
 
 section DerivingSemantics
 
-def VeilM.canRaise (ex : Set ExId) (act : VeilM m σ ρ α) (pre : SProp ρ σ) : Prop :=
+def VeilM.canRaise (ex : Set ExId) (act : VeilM m ρ σ α) (pre : SProp ρ σ) : Prop :=
   [CanRaise ex| triple pre act (fun _ => ⊤)]
 
-def VeilSpecM.toTwoStateDerived (spec : VeilSpecM σ ρ α) : TwoState ρ σ :=
+def VeilSpecM.toTwoStateDerived (spec : VeilSpecM ρ σ α) : TwoState ρ σ :=
   fun r₀ s₀ s₁ => spec.inv (fun _ r s => r = r₀ ∧ s = s₁) r₀ s₀
 
-def VeilM.toTwoStateDerived (act : VeilM m σ ρ α) : TwoState ρ σ :=
+def VeilM.toTwoStateDerived (act : VeilM m ρ σ α) : TwoState ρ σ :=
   [CanRaise (fun _ => True)| VeilSpecM.toTwoStateDerived <| wp act]
 
 end DerivingSemantics
