Veil/Theory/WP.lean
@@ -57,34 +57,34 @@ instance (priority := high + 1) [IsSubStateOf σₛ σ] [Monad m] : MonadReaderO
 
 /- Languge constructs -/
 
-def VeilExecM.assert (p : Prop) [Decidable p] (ex : ExId) : VeilExecM m σ ρ Unit := do
+def VeilExecM.assert (p : Prop) [Decidable p] (ex : ExId) : VeilExecM m ρ σ Unit := do
   if p then pure () else throw ex
 
-def VeilM.assert (p : Prop) [Decidable p] (ex : ExId) : VeilM m σ ρ Unit := do
-  liftM (@VeilExecM.assert m σ ρ p _ ex)
+def VeilM.assert (p : Prop) [Decidable p] (ex : ExId) : VeilM m ρ σ Unit := do
+  liftM (@VeilExecM.assert m ρ σ p _ ex)
 
-def VeilM.require (p : Prop) [Decidable p] (ex : ExId) : VeilM m σ ρ Unit := do
+def VeilM.require (p : Prop) [Decidable p] (ex : ExId) : VeilM m ρ σ Unit := do
   match m with
   | .internal => VeilM.assert p ex
   | .external => assume p
 
 @[wpSimp]
 lemma VeilExecM.wp_assume :
-  wp (assume p : VeilM m σ ρ PUnit) post = fun r s => p -> post .unit r s := by
+  wp (assume p : VeilM m ρ σ PUnit) post = fun r s => p -> post .unit r s := by
   simp [MonadNonDet.wp_assume, loomLogicSimp, himp];
 
 @[wpSimp]
 lemma VeilM.wp_require (p : Prop) [Decidable p] (ex : ExId) :
-  wp (require p ex : VeilM m σ ρ Unit) post =
+  wp (require p ex : VeilM m ρ σ Unit) post =
     match m with
-    | .internal => wp (VeilM.assert p ex : VeilM m σ ρ Unit) post
-    | .external => wp (assume p : VeilM m σ ρ PUnit) post := by
+    | .internal => wp (VeilM.assert p ex : VeilM m ρ σ Unit) post
+    | .external => wp (assume p : VeilM m ρ σ PUnit) post := by
   cases m <;> rfl
 
 
 @[wpSimp]
 lemma VeilExecM.wp_assert (p : Prop) [Decidable p] (ex : ExId) :
-  wp (@VeilExecM.assert m σ ρ p _ ex) post = fun r s => if p then post () r s else hd ex := by
+  wp (@VeilExecM.assert m ρ σ p _ ex) post = fun r s => if p then post () r s else hd ex := by
   simp [VeilExecM.assert]; split
   { simp [wp_pure] }
   simp [throw, throwThe, ReaderT.instMonadExceptOf, StateT.instMonadExceptOf]
@@ -95,40 +95,40 @@ lemma VeilExecM.wp_assert (p : Prop) [Decidable p] (ex : ExId) :
 
 @[wpSimp]
 lemma VeilM.wp_assert (p : Prop) [Decidable p] (ex : ExId) :
-  wp (@VeilM.assert m σ ρ p _ ex) post = fun r s => if p then post () r s else hd ex := by
+  wp (@VeilM.assert m ρ σ p _ ex) post = fun r s => if p then post () r s else hd ex := by
   simp [VeilM.assert, MPropLift.wp_lift, wpSimp]
 
 @[wpSimp]
 lemma VeilM.wp_get [IsSubStateOf σₛ σ] :
-  wp (get : VeilM m σ ρ σₛ) post = fun r s => post (getFrom s) r s := by
+  wp (get : VeilM m ρ σ σₛ) post = fun r s => post (getFrom s) r s := by
   simp [get, getThe, MonadStateOf.get, MPropLift.wp_lift]; ext
   erw [StateT.wp_get]
 
 @[wpSimp]
 lemma VeilM.wp_modifyGet [IsSubStateOf σₛ σ] :
-  wp (modifyGet f : VeilM m σ ρ σₛ) post = fun r s => post (f (getFrom s)).1 r (setIn (f (getFrom s)).2 s) := by
+  wp (modifyGet f : VeilM m ρ σ σₛ) post = fun r s => post (f (getFrom s)).1 r (setIn (f (getFrom s)).2 s) := by
   simp [modifyGet, MonadStateOf.modifyGet, MPropLift.wp_lift]; ext
   erw [StateT.wp_modifyGet]
 
 @[wpSimp]
 lemma VeilExecM.wp_read [IsSubStateOf ρₛ ρ] :
-  wp (read : VeilExecM m σ ρ ρₛ) post = fun r s => post (getFrom r) r s := by
+  wp (read : VeilExecM m ρ σ ρₛ) post = fun r s => post (getFrom r) r s := by
   simp [read, getThe, MonadReaderOf.read, MPropLift.wp_lift]; ext
   erw [ReaderT.wp_read]
 
 @[wpSimp]
 lemma VeilM.wp_pick :
-  wp (pick τ : VeilM m σ ρ τ) post = fun r s => ∀ t, post t r s := by
+  wp (pick τ : VeilM m ρ σ τ) post = fun r s => ∀ t, post t r s := by
   simp [MonadNonDet.wp_pick, loomLogicSimp, himp, iInf, sInf]; aesop
 
 @[wpSimp]
 lemma VeilM.wp_pickSuchThat :
-  wp (pickSuchThat τ p : VeilM m σ ρ τ) post = fun r s => ∀ t, p t -> post t r s := by
+  wp (pickSuchThat τ p : VeilM m ρ σ τ) post = fun r s => ∀ t, p t -> post t r s := by
   simp [MonadNonDet.wp_pickSuchThat, loomLogicSimp, himp, iInf, sInf]; aesop
 
 @[wpSimp]
 lemma VeilM.wp_if [Decidable p] :
-  wp (if p then a else b : VeilM m σ ρ τ) post =
+  wp (if p then a else b : VeilM m ρ σ τ) post =
   if p then wp a post else wp b post := by
   split_ifs <;> simp
 
