Test/BasicSyntax.lean
@@ -10,16 +10,41 @@ relation r : node -> Nat -> Prop
 individual n : node
 function f : Nat -> Nat
 
+set_option trace.veil.debug true
+
 #gen_state
-#guard_msgs(drop warning) in
+
+#check VeilM.require
+
+-- set_option pp.all true
+
+-- #guard_msgs(drop warning) in
 action foo (k : Nat) =
-  requires ∀ x, r x k
-  ensures True
+  -- requires ∀ x, r x k
+  -- ensures True
 {
   let x <- pick node
   -- return x
   require r x k
 }
+
+#print foo.wpSucc_eq
+
+#print foo.ext.wp_eq
+
+#check foo.wp_eq
+
+open PartialCorrectness DemonicChoice
+
+example (P : _ -> Prop) (hd : ExId -> Prop) [IsHandler hd]
+  [σ_substate : IsSubStateOf (State node) σ] [ρ_reader : IsSubStateOf (Reader node σ) ρ] :
+  P ( Test.foo.ext.wpSucc (σ_substate := σ_substate) (ρ_reader := ρ_reader)) := by
+  unfold Test.foo.ext.wpSucc
+  simp [actSimp]
+
+
+
+#print foo.ext.gen_wp
 
 
 #guard_msgs(drop warning) in
